Updates.

FOL/NV/Deduct.lean
@@ -74,6 +74,9 @@ def is_prop_proof (phi : Formula_) : Prop :=
   is_prop_deduct ∅ phi
 
 
+-------------------------------------------------------------------------------
+
+
 /--
   `is_axiom_v1 F` := True if and only if `F` is an axiom of classical first order logic.
 -/
@@ -204,6 +207,67 @@ def is_proof_v1 (F : Formula_) : Prop :=
   is_deduct_v1 ∅ F
 
 
+-------------------------------------------------------------------------------
+
+
+lemma is_prop_axiom_imp_is_axiom_v1
+  (F : Formula_)
+  (h1 : is_prop_axiom F) :
+  is_axiom_v1 F :=
+  by
+  induction h1
+  case prop_true_ =>
+    apply is_axiom_v1.prop_true_
+  case prop_1_ phi psi =>
+    apply is_axiom_v1.prop_1_
+  case prop_2_ phi psi chi =>
+    apply is_axiom_v1.prop_2_
+  case prop_3_ phi psi =>
+    apply is_axiom_v1.prop_3_
+  case def_false_ =>
+    apply is_axiom_v1.def_false_
+  case def_and_ phi psi =>
+    apply is_axiom_v1.def_and_
+  case def_or_ phi psi =>
+    apply is_axiom_v1.def_or_
+  case def_iff_ phi psi =>
+    apply is_axiom_v1.def_iff_
+
+
+lemma is_prop_deduct_imp_is_deduct_v1
+  (Δ : Set Formula_)
+  (F : Formula_)
+  (h1 : is_prop_deduct Δ F) :
+  is_deduct_v1 Δ F :=
+  by
+  induction h1
+  case axiom_ phi ih =>
+    apply is_deduct_v1.axiom_
+    apply is_prop_axiom_imp_is_axiom_v1
+    exact ih
+  case assume_ phi ih =>
+    apply is_deduct_v1.assume_
+    exact ih
+  case mp_ phi psi ih_1 ih_2 ih_3 ih_4 =>
+    apply is_deduct_v1.mp_ phi
+    · exact ih_3
+    · exact ih_4
+
+
+lemma is_prop_proof_imp_is_proof_v1
+  (F : Formula_)
+  (h1 : is_prop_proof F) :
+  is_proof_v1 F :=
+  by
+  unfold is_prop_proof at h1
+  unfold is_proof_v1
+  apply is_prop_deduct_imp_is_deduct_v1
+  exact h1
+
+
+-------------------------------------------------------------------------------
+
+
 /--
   `is_proof_v2 F` := True if and only if there is a proof of `F` in classical first order logic.
 
@@ -321,59 +385,236 @@ inductive is_proof_v2 : Formula_ → Prop
     is_proof_v2 ((exists_ v phi).iff_ (not_ (forall_ v (not_ phi))))
 
 
-lemma is_prop_axiom_imp_is_axiom_v1
+-------------------------------------------------------------------------------
+
+
+inductive is_axiom_v3 : Formula_ → Prop
+  -- `⊢ ⊤`
+  | prop_true_ :
+    is_axiom_v3 true_
+
+  -- `⊢ phi → (psi → phi)`
+  | prop_1_
+    (phi psi : Formula_) :
+    is_axiom_v3 (phi.imp_ (psi.imp_ phi))
+
+  -- `⊢ (phi → (psi → chi)) → ((phi → psi) → (phi → chi))`
+  | prop_2_
+    (phi psi chi : Formula_) :
+    is_axiom_v3 ((phi.imp_ (psi.imp_ chi)).imp_ ((phi.imp_ psi).imp_ (phi.imp_ chi)))
+
+  -- `⊢ (¬ phi → ¬ psi) → (psi → phi)`
+  | prop_3_
+    (phi psi : Formula_) :
+    is_axiom_v3 (((not_ phi).imp_ (not_ psi)).imp_ (psi.imp_ phi))
+
+  -- `⊢ (∀ v (phi → psi)) → ((∀ v phi) → (∀ v psi))`
+  | pred_1_
+    (v : VarName_)
+    (phi psi : Formula_) :
+    is_axiom_v3 ((forall_ v (phi.imp_ psi)).imp_ ((forall_ v phi).imp_ (forall_ v psi)))
+
+  -- `⊢ (∀ v phi) → phi(t/v)` provided `phi` admits `t` for `v`
+  | pred_2_
+    (v t : VarName_)
+    (phi phi' : Formula_) :
+    FOL.NV.Sub.Var.One.Rec.fast_admits_var_one_rec v t phi →
+    FOL.NV.Sub.Var.One.Rec.fast_replace_free_var_one_rec v t phi = phi' →
+    is_axiom_v3 ((forall_ v phi).imp_ phi')
+
+  -- `⊢ phi → (∀ v phi)` provided `v` is not free in `phi`
+  | pred_3_
+    (v : VarName_)
+    (phi : Formula_) :
+    ¬ var_is_free_in v phi →
+    is_axiom_v3 (phi.imp_ (forall_ v phi))
+
+  -- `⊢ ∀ v (v = v)`
+  | eq_1_ (v : VarName_) :
+    is_axiom_v3 (forall_ v (eq_ v v))
+
+  /-
+    `⊢ ∀ x_0 ... ∀ x_n ∀ y_0 ... y_n ((x_0 = y_0) ∧ ... ∧ (x_n = y_n) ∧ ⊤) →((pred_ name [x_0 ... x_n] ↔ pred_ name [y_0 ... y_n]))`
+  -/
+  | eq_2_pred_const_
+    (name : PredName_)
+    (xs ys : List VarName_) :
+    xs.length = ys.length →
+    is_axiom_v3
+      (Forall_ xs
+        (Forall_ ys
+          ((And_ (List.zipWith eq_ xs ys)).imp_
+            ((pred_const_ name xs).iff_ (pred_const_ name ys)))))
+
+  /-
+    `⊢ ∀ x_0 ∀ x_1 ∀ y_0 ∀ y_1 ((x_0 = y_0) ∧ (x_1 = y_1)) → ((eq_ x_0 x_1) ↔ (eq_ y_0 y_1))`
+  -/
+  | eq_2_eq_
+    (x_0 x_1 y_0 y_1 : VarName_) :
+    is_axiom_v3
+      (forall_ x_0
+        (forall_ x_1
+          (forall_ y_0
+            (forall_ y_1
+              ((and_ (eq_ x_0 y_0) (eq_ x_1 y_1)).imp_
+                ((eq_ x_0 x_1).iff_ (eq_ y_0 y_1)))))))
+
+  -- `⊢ phi ⇒ ⊢ ∀ v phi`
+  | gen_
+    (v : VarName_)
+    (phi : Formula_) :
+    is_axiom_v3 phi →
+    is_axiom_v3 (forall_ v phi)
+
+  | def_false_ :
+    is_axiom_v3 (false_.iff_ (not_ true_))
+
+  | def_and_
+    (phi psi : Formula_) :
+    is_axiom_v3 ((phi.and_ psi).iff_ (not_ (phi.imp_ (not_ psi))))
+
+  | def_or_
+    (phi psi : Formula_) :
+    is_axiom_v3 ((phi.or_ psi).iff_ ((not_ phi).imp_ psi))
+
+  | def_iff_
+    (phi psi : Formula_) :
+    is_axiom_v3 (not_ (((phi.iff_ psi).imp_ (not_ ((phi.imp_ psi).imp_ (not_ (psi.imp_ phi))))).imp_ (not_ ((not_ ((phi.imp_ psi).imp_ (not_ (psi.imp_ phi)))).imp_ (phi.iff_ psi)))))
+
+  | def_exists_
+    (v : VarName_)
+    (phi : Formula_) :
+    is_axiom_v3 ((exists_ v phi).iff_ (not_ (forall_ v (not_ phi))))
+
+
+theorem extracted_1
+  {α β : Type}
+  (f : α → α → β)
+  (n : ℕ)
+  (xs ys : Fin n → α) :
+  List.ofFn (fun (i : Fin n) => f (xs i) (ys i)) = List.zipWith f (List.ofFn xs) (List.ofFn ys) :=
+  by
+    induction n
+    case zero =>
+      simp
+    case succ m ih =>
+      simp
+      exact ih (fun i => xs i.succ) fun i => ys i.succ
+
+
+theorem extracted_2
+  {α β : Type}
+  (f : α → α → β)
+  (xs ys : List α)
+  (h1 : xs.length = ys.length) :
+  (List.ofFn fun (i : Fin xs.length) => f xs[↑i] ys[↑i]) = List.zipWith f xs ys :=
+  by
+  induction xs generalizing ys
+  case nil =>
+    simp
+  case cons xs_hd xs_tl xs_ih =>
+    cases ys
+    case nil =>
+      simp at h1
+    case cons ys_hd ys_tl =>
+      simp at h1
+
+      simp
+      apply xs_ih
+      exact h1
+
+
+theorem extracted_4
+  {α β : Type}
+  (f : α → α → β)
+  (xs_hd : α)
+  (xs_tl : List α)
+  (ys_hd : α)
+  (ys_tl : List α) :
+  (List.ofFn (fun (i : Fin (min (xs_hd :: xs_tl).length (ys_hd :: ys_tl).length)) => f (xs_hd :: xs_tl)[i] (ys_hd :: ys_tl)[i])) =
+  f xs_hd ys_hd :: List.ofFn (fun (i : Fin (min xs_tl.length ys_tl.length)) => f xs_tl[i] ys_tl[i]) :=
+  by
+    ext n z
+    induction n
+    case _ =>
+      simp
+    case _ n ih =>
+      simp
+      simp only [List.ofFnNthVal]
+      simp
+
+
+lemma extracted_5
+  {α β : Type}
+  (f : α → α → β)
+  (xs ys : List α) :
+  (List.ofFn (fun (i : Fin (min xs.length ys.length)) => f xs[↑i] ys[↑i])) = List.zipWith f xs ys :=
+  by
+  induction xs generalizing ys
+  case nil =>
+    simp
+  case cons xs_hd xs_tl xs_ih =>
+    cases ys
+    case nil =>
+      simp
+    case cons ys_hd ys_tl =>
+      simp only [List.zipWith]
+      rw [extracted_4]
+      congr
+      apply xs_ih
+
+
+lemma extracted_3
+  {α β : Type}
+  (f : α → α → β)
+  (xs ys : List α)
+  (h1 : xs.length = ys.length) :
+  ∃ (n : Nat) (fn_xs fn_ys : Fin n → α),
+    List.ofFn (fun i => f (fn_xs i) (fn_ys i)) = List.zipWith f xs ys ∧
+    List.ofFn fn_xs = xs ∧
+    List.ofFn fn_ys = ys :=
+  by
+    apply Exists.intro (xs.length)
+    apply Exists.intro (fun i => xs[i])
+    apply Exists.intro (fun i => ys[i])
+    constructor
+    · simp
+      apply extracted_2
+      exact h1
+    · constructor
+      . simp
+      · simp [h1]
+
+
+example
   (F : Formula_)
-  (h1 : is_prop_axiom F) :
+  (h1 : is_axiom_v1 F) :
+  is_axiom_v3 F :=
+  by
+  induction h1
+  case eq_2_pred_const_ name n xs ys =>
+    rw [extracted_1]
+    apply is_axiom_v3.eq_2_pred_const_
+    simp
+  all_goals
+    sorry
+
+
+example
+  (F : Formula_)
+  (h1 : is_axiom_v3 F) :
   is_axiom_v1 F :=
   by
   induction h1
-  case prop_true_ =>
-    apply is_axiom_v1.prop_true_
-  case prop_1_ phi psi =>
-    apply is_axiom_v1.prop_1_
-  case prop_2_ phi psi chi =>
-    apply is_axiom_v1.prop_2_
-  case prop_3_ phi psi =>
-    apply is_axiom_v1.prop_3_
-  case def_false_ =>
-    apply is_axiom_v1.def_false_
-  case def_and_ phi psi =>
-    apply is_axiom_v1.def_and_
-  case def_or_ phi psi =>
-    apply is_axiom_v1.def_or_
-  case def_iff_ phi psi =>
-    apply is_axiom_v1.def_iff_
+  case eq_2_pred_const_ name xs ys ih =>
+    obtain ⟨n, fn_xs, fn_ys, c1, c2, c3⟩ := extracted_3 eq_ xs ys ih
+    rw [← c1]
+    rw [← c2]
+    rw [← c3]
+
+    apply is_axiom_v1.eq_2_pred_const_
+  all_goals
+    sorry
 
 
-lemma is_prop_deduct_imp_is_deduct_v1
-  (Δ : Set Formula_)
-  (F : Formula_)
-  (h1 : is_prop_deduct Δ F) :
-  is_deduct_v1 Δ F :=
-  by
-  induction h1
-  case axiom_ phi ih =>
-    apply is_deduct_v1.axiom_
-    apply is_prop_axiom_imp_is_axiom_v1
-    exact ih
-  case assume_ phi ih =>
-    apply is_deduct_v1.assume_
-    exact ih
-  case mp_ phi psi ih_1 ih_2 ih_3 ih_4 =>
-    apply is_deduct_v1.mp_ phi
-    · exact ih_3
-    · exact ih_4
-
-
-lemma is_prop_proof_imp_is_proof_v1
-  (F : Formula_)
-  (h1 : is_prop_proof F) :
-  is_proof_v1 F :=
-  by
-  unfold is_prop_proof at h1
-  unfold is_proof_v1
-  apply is_prop_deduct_imp_is_deduct_v1
-  exact h1
-
-
-#lint
+--#lint
