FOL/NV/Pred.lean
@@ -1,4 +1,5 @@
 import FOL.NV.Prop
+import FOL.NV.ReplaceSubFormula
 
 
 set_option autoImplicit false
@@ -8,13 +9,6 @@ open Formula_
 
 open FOL.NV.Sub.Var.One.Rec
 
-
-axiom def_false_ : false_ = not_ true_
-
-/--
-  phi ∨ psi := ¬ phi → psi
--/
-axiom def_or_ (phi psi : Formula_) : or_ phi psi = (not_ phi).imp_ psi
 
 /--
 phi ∧ psi := ¬ ( phi → ¬ psi )
@@ -31,14 +25,12 @@ axiom def_iff_ (phi psi : Formula_) : iff_ phi psi = (phi.imp_ psi).and_ (psi.im
 -/
 axiom def_exists_ (x : VarName_) (phi : Formula_) : exists_ x phi = not_ (forall_ x (not_ phi))
 
+
 def def_eq_ (x y : VarName_) : Formula_ :=
   pred_const_ (PredName_.mk "=") [x, y]
 
 
-def ProofEquiv (P Q : Formula_) : Prop :=
-  is_proof_v1 (P.iff_ Q)
-
-
+/-
 /--
   IsReplOfVarInListFun u v l_u l_v := True if and only if l_v is the result of replacing one or more specified occurrences (but not necessarily all occurrences) of u in l_u by occurrences of v.
 -/
@@ -307,9 +299,10 @@ inductive IsReplOfFormulaInFormula
     (P_u P_v : Formula_) :
     IsReplOfFormulaInFormula U V P_u P_v →
     IsReplOfFormulaInFormula U V (exists_ x P_u) (exists_ x P_v)
+-/
 
 
-def Similar
+def similar
   (P_u P_v : Formula_)
   (u v : VarName_) :
   Prop :=
@@ -338,7 +331,7 @@ alias spec := T_17_1
 alias forall_elim := T_17_1
 
 
-theorem specId
+theorem spec_id
   (v : VarName_)
   (P : Formula_)
   (Δ : Set Formula_)
@@ -348,11 +341,11 @@ theorem specId
   apply is_deduct_v1.mp_ (forall_ v P)
   · apply is_deduct_v1.axiom_
     apply is_axiom_v1.pred_2_ v v P
-    · exact fast_admits_var_one_rec_self P v
-    · exact fast_replace_free_var_one_rec_self P v
+    · apply fast_admits_var_one_rec_self
+    · apply fast_replace_free_var_one_rec_self
   · exact h1
 
-alias forall_elim_id := specId
+alias forall_elim_id := spec_id
 
 
 theorem T_17_3
@@ -395,7 +388,7 @@ theorem T_17_4
 alias exists_intro := T_17_4
 
 
-theorem existsIntroId
+theorem exists_intro_id
   (P : Formula_)
   (v : VarName_)
   (Δ : Set Formula_)
@@ -403,7 +396,7 @@ theorem existsIntroId
   is_deduct_v1 Δ (exists_ v P) :=
   by
   apply T_17_4 P v v Δ
-  · exact fast_admits_var_one_rec_self P v
+  · apply fast_admits_var_one_rec_self
   · simp only [fast_replace_free_var_one_rec_self]
     exact h1
 
@@ -415,8 +408,8 @@ theorem T_17_6
   by
   apply deduction_theorem
   simp
-  apply existsIntroId
-  apply specId v
+  apply exists_intro_id
+  apply spec_id v
   apply is_deduct_v1.assume_
   simp
 
@@ -453,7 +446,7 @@ alias generalization := T_17_7
 
 
 -- Universal Introduction
-theorem univIntro
+theorem univ_intro
   (P : Formula_)
   (v t : VarName_)
   (Δ : Set Formula_)
@@ -481,11 +474,12 @@ theorem univIntro
   · exact generalization (fast_replace_free_var_one_rec v t P) t Δ h2 h3
 
 
-theorem isProofAltImpIsDeduct
+theorem is_proof_v2_imp_is_proof_v1
   (F : Formula_)
   (h1 : is_proof_v2 F) :
-  is_deduct_v1 ∅ F :=
+  is_proof_v1 F :=
   by
+  unfold is_proof_v1
   induction h1
   case prop_true_ =>
     apply is_deduct_v1.axiom_
@@ -541,11 +535,12 @@ theorem isProofAltImpIsDeduct
     apply is_axiom_v1.def_exists_
 
 
-theorem isDeductImpIsProofAlt
+theorem is_proof_v1_imp_is_proof_v2
   (F : Formula_)
-  (h1 : is_deduct_v1 ∅ F) :
+  (h1 : is_proof_v1 F) :
   is_proof_v2 F :=
   by
+  unfold is_proof_v1 at h1
   induction h1
   case axiom_ h1_phi h1_1 =>
     induction h1_1
@@ -598,8 +593,8 @@ theorem T_17_10
   simp
   apply generalization
   · apply generalization
-    · apply specId v P
-      apply specId u (forall_ v P)
+    · apply spec_id v P
+      apply spec_id u (forall_ v P)
       apply is_deduct_v1.assume_
       simp
     · simp
@@ -619,7 +614,6 @@ theorem T_17_11
   apply deduction_theorem
   simp
   simp only [def_exists_]
-  -- simp only [exists_]
   apply is_deduct_v1.mp_ (Q.not_.imp_ (forall_ v Q.not_))
   · apply is_deduct_v1.mp_ ((forall_ v Q.not_).imp_ (forall_ v P.not_))
     · SC
@@ -630,7 +624,7 @@ theorem T_17_11
         · apply is_deduct_v1.mp_ (P.imp_ Q)
           · apply proof_imp_deduct
             apply T_14_7
-          · apply specId v (P.imp_ Q)
+          · apply spec_id v (P.imp_ Q)
             apply is_deduct_v1.assume_
             simp
         · simp
@@ -667,7 +661,7 @@ alias rule_C := T_17_12
 
 
 -- Existential Elimination
-theorem existsElim
+theorem exists_elim
   (P Q : Formula_)
   (v t : VarName_)
   (Δ : Set Formula_)
@@ -679,22 +673,20 @@ theorem existsElim
   by
   refine' rule_C (fast_replace_free_var_one_rec v t P) Q t Δ _ h2 h5 _
   · simp only [def_exists_] at h1
-    -- simp only [exists_] at h1
     simp only [def_exists_]
-    -- simp only [exists_]
     apply is_deduct_v1.mp_ (forall_ v P.not_).not_
     · apply is_deduct_v1.mp_ ((forall_ t (fast_replace_free_var_one_rec v t P.not_)).imp_ (forall_ v P.not_))
       · SC
       · apply deduction_theorem
-        apply univIntro P.not_ v t _ h3
-        · apply specId t
+        apply univ_intro P.not_ v t _ h3
+        · apply spec_id t
           apply is_deduct_v1.assume_
           simp
         · intro H a1
           simp at a1
           cases a1
           case _ c1 =>
-            subst c1
+            rw [c1]
             simp only [var_is_free_in]
             simp
           case _ c1 =>
@@ -719,14 +711,12 @@ theorem T_17_14
   · apply is_deduct_v1.mp_ (exists_ v Q)
     · apply is_deduct_v1.mp_ (exists_ v P)
       · simp only [def_and_]
-        -- simp only [formula.and_]
         SC
       · apply exists_intro P v v
         · apply fast_admits_var_one_rec_self
         · simp only [fast_replace_free_var_one_rec_self]
           apply is_deduct_v1.mp_ (P.and_ Q)
           · simp only [def_and_]
-            -- simp only [formula.and_]
             SC
           · apply is_deduct_v1.assume_
             simp
@@ -735,21 +725,16 @@ theorem T_17_14
       · simp only [fast_replace_free_var_one_rec_self]
         apply is_deduct_v1.mp_ (P.and_ Q)
         · simp only [def_and_]
-          -- simp only [formula.and_]
           SC
         · apply is_deduct_v1.assume_
           simp
   · simp only [def_and_]
-    -- simp only [and_]
     simp only [def_exists_]
-    -- simp only [exists_]
     simp
     simp only [var_is_free_in]
     simp
   · simp only [def_and_]
-    -- simp only [and_]
     simp only [def_exists_]
-    -- simp only [exists_]
     simp only [var_is_free_in]
     simp
 
@@ -760,7 +745,6 @@ theorem T_18_1_left
   is_proof_v1 ((forall_ v (P.iff_ Q)).imp_ ((forall_ v P).imp_ (forall_ v Q))) :=
   by
   simp only [def_iff_]
-  -- simp only [iff_]
   apply deduction_theorem
   apply deduction_theorem
   simp
@@ -768,12 +752,11 @@ theorem T_18_1_left
   · apply is_deduct_v1.mp_ P
     · apply is_deduct_v1.mp_ ((P.imp_ Q).and_ (Q.imp_ P))
       · simp only [def_and_]
-        -- simp only [formula.and_]
         SC
-      · apply specId v
+      · apply spec_id v
         apply is_deduct_v1.assume_
         simp
-    · apply specId v
+    · apply spec_id v
       apply is_deduct_v1.assume_
       simp
   · simp
@@ -787,7 +770,6 @@ theorem T_18_1_right
   is_proof_v1 ((forall_ v (P.iff_ Q)).imp_ ((forall_ v Q).imp_ (forall_ v P))) :=
   by
   simp only [def_iff_]
-  -- simp only [iff_]
   apply deduction_theorem
   apply deduction_theorem
   simp
@@ -795,12 +777,11 @@ theorem T_18_1_right
   · apply is_deduct_v1.mp_ Q
     · apply is_deduct_v1.mp_ ((P.imp_ Q).and_ (Q.imp_ P))
       · simp only [def_and_]
-        -- simp only [formula.and_]
         SC
-      · apply specId v
+      · apply spec_id v
         apply is_deduct_v1.assume_
         simp
-    · apply specId v
+    · apply spec_id v
       apply is_deduct_v1.assume_
       simp
   · simp
@@ -816,9 +797,7 @@ theorem T_18_1
   apply is_deduct_v1.mp_ ((forall_ v (P.iff_ Q)).imp_ ((forall_ v Q).imp_ (forall_ v P)))
   · apply is_deduct_v1.mp_ ((forall_ v (P.iff_ Q)).imp_ ((forall_ v P).imp_ (forall_ v Q)))
     · simp only [def_iff_]
-      -- simp only [formula.iff_]
       simp only [def_and_]
-      -- simp only [formula.and_]
       SC
     · apply T_18_1_left
   · apply T_18_1_right
@@ -838,12 +817,12 @@ theorem Forall_spec_id
     apply deduction_theorem
     simp
     apply is_deduct_v1.mp_ (Forall_ xs_tl P)
-    apply proof_imp_deduct
-    exact xs_ih
-    apply specId xs_hd
-    apply is_deduct_v1.assume_
-    simp
-    rfl
+    · apply proof_imp_deduct
+      exact xs_ih
+    · apply spec_id xs_hd
+      apply is_deduct_v1.assume_
+      simp
+      rfl
 
 
 theorem Forall_spec_id'
@@ -863,11 +842,11 @@ theorem Forall_spec_id'
     simp at h1
     apply xs_ih
     simp only [Forall_]
-    apply specId xs_hd
+    apply spec_id xs_hd
     exact h1
 
 
-theorem Forall_isBoundIn
+theorem Forall_var_is_bound_in
   (P : Formula_)
   (xs : List VarName_)
   (x : VarName_) :
@@ -884,7 +863,7 @@ theorem Forall_isBoundIn
     tauto
 
 
-theorem Forall_isFreeIn
+theorem Forall_var_is_free_in
   (P : Formula_)
   (xs : List VarName_)
   (x : VarName_) :
@@ -906,7 +885,7 @@ theorem T_18_2
   (U V : Formula_)
   (P_U P_V : Formula_)
   (l : List VarName_)
-  (h1 : IsReplOfFormulaInFormula U V P_U P_V)
+  (h1 : is_repl_of_formula_in_formula U V P_U P_V)
   (h2 : ∀ (v : VarName_), (var_is_free_in v U ∨ var_is_free_in v V) ∧ var_is_bound_in v P_U → v ∈ l) :
   is_proof_v1 ((Forall_ l (U.iff_ V)).imp_ (P_U.iff_ P_V)) :=
   by
@@ -914,21 +893,17 @@ theorem T_18_2
   case same_ h1_P h1_P' h1_1 =>
     subst h1_1
     simp only [def_iff_]
-    -- simp only [formula.iff_]
     simp only [def_and_]
-    -- simp only [formula.and_]
     SC
   case diff_ h1_P h1_P' h1_1 h1_2 =>
-    subst h1_1
-    subst h1_2
+    rw [h1_1]
+    rw [h1_2]
     apply Forall_spec_id
   case not_ h1_P h1_P' h1_1 h1_ih =>
     simp only [var_is_bound_in] at h2
     apply is_deduct_v1.mp_ ((Forall_ l (U.iff_ V)).imp_ (h1_P.iff_ h1_P'))
     · simp only [def_iff_]
-      -- simp only [formula.iff_]
       simp only [def_and_]
-      -- simp only [formula.and_]
       SC
     · exact h1_ih h2
   case imp_ h1_P h1_Q h1_P' h1_Q' h1_1 h1_2 h1_ih_1 h1_ih_2 =>
@@ -936,9 +911,7 @@ theorem T_18_2
     apply is_deduct_v1.mp_ ((Forall_ l (U.iff_ V)).imp_ (h1_P.iff_ h1_P'))
     · apply is_deduct_v1.mp_ ((Forall_ l (U.iff_ V)).imp_ (h1_Q.iff_ h1_Q'))
       · simp only [def_iff_]
-        -- simp only [formula.iff_]
         simp only [def_and_]
-        -- simp only [formula.and_]
         SC
       · apply h1_ih_2
         intro v a2
@@ -947,50 +920,50 @@ theorem T_18_2
     · apply h1_ih_1
       intro v a1
       apply h2 v
-      cases a1
-      case _ a1_left a1_right =>
-        constructor
-        · exact a1_left
-        · left
-          exact a1_right
-  case forall_ h1_x h1_P h1_P' h1_1 h1_ih =>
+      obtain ⟨a1_left, a1_right⟩ := a1
+      constructor
+      · exact a1_left
+      · left
+        exact a1_right
+  case forall_ h1_u h1_v h1_P_U h1_P_V h1_ih_1 h1_ih_2 h1_ih_3 =>
+    rw [h1_ih_1]
+
     simp only [var_is_bound_in] at h2
     simp at h2
+
     apply deduction_theorem
     simp
-    apply is_deduct_v1.mp_ (forall_ h1_x (h1_P.iff_ h1_P'))
+    apply is_deduct_v1.mp_ (forall_ h1_v (h1_P_U.iff_ h1_P_V))
     · apply proof_imp_deduct
       apply T_18_1
     · apply generalization
       · apply is_deduct_v1.mp_ (Forall_ l (U.iff_ V))
         · apply proof_imp_deduct
-          apply h1_ih
+          apply h1_ih_3
           intro v a1
-          cases a1
-          case _ a1_left a1_right =>
-            apply h2 v a1_left
-            right
-            apply a1_right
+          obtain ⟨a1_left, a1_right⟩ := a1
+          apply h2 v a1_left
+          right
+          apply a1_right
         · apply is_deduct_v1.assume_
           simp
       · intro H a1
         simp at a1
-        subst a1
-        simp only [Forall_isFreeIn]
+        rw [a1]
+        simp only [Forall_var_is_free_in]
         simp only [def_iff_]
-        -- simp only [formula.iff_]
         simp only [def_and_]
-        -- simp only [formula.and_]
         simp only [var_is_free_in]
         simp
         contrapose
-        push_neg
+        simp
         intro a2
         apply h2
         simp_all
         · tauto
         · left
-          rfl
+          symm
+          exact h1_ih_1
   all_goals
     sorry
 
@@ -998,12 +971,11 @@ theorem T_18_2
 theorem C_18_3
   (U V : Formula_)
   (P_U P_V : Formula_)
-  (h1 : IsReplOfFormulaInFormula U V P_U P_V)
-  (h2 : is_proof_v1 (U.iff_ V)) : is_proof_v1 (P_U.iff_ P_V) :=
+  (h1 : is_repl_of_formula_in_formula U V P_U P_V)
+  (h2 : is_proof_v1 (U.iff_ V)) :
+  is_proof_v1 (P_U.iff_ P_V) :=
   by
-  apply
-    is_deduct_v1.mp_
-      (Forall_ ((U.free_var_set ∪ V.free_var_set) ∩ P_U.bound_var_set).toList (U.iff_ V))
+  apply is_deduct_v1.mp_ (Forall_ ((U.free_var_set ∪ V.free_var_set) ∩ P_U.bound_var_set).toList (U.iff_ V))
   · apply T_18_2 U V P_U P_V ((U.free_var_set ∪ V.free_var_set) ∩ P_U.bound_var_set).toList h1
     intro v a1
     simp
@@ -1027,7 +999,7 @@ theorem C_18_4
   (U V : Formula_)
   (P_U P_V : Formula_)
   (Δ : Set Formula_)
-  (h1 : IsReplOfFormulaInFormula U V P_U P_V)
+  (h1 : is_repl_of_formula_in_formula U V P_U P_V)
   (h2 : is_proof_v1 (U.iff_ V))
   (h3 : is_deduct_v1 Δ P_U) :
   is_deduct_v1 Δ P_V :=
@@ -1036,8 +1008,6 @@ theorem C_18_4
   · apply is_deduct_v1.mp_ (P_U.iff_ P_V)
     · simp only [def_iff_]
       simp only [def_and_]
-      -- simp only [formula.iff_]
-      -- simp only [formula.and_]
       SC
     · apply proof_imp_deduct
       exact C_18_3 U V P_U P_V h1 h2
@@ -1050,99 +1020,84 @@ theorem T_18_5
   is_proof_v1 ((forall_ v P).iff_ (exists_ v P.not_).not_) :=
   by
   simp only [def_exists_]
-  -- simp only [exists_]
   apply C_18_4 P P.not_.not_ ((forall_ v P).iff_ (forall_ v P).not_.not_)
   · simp only [def_iff_]
     simp only [def_and_]
-    -- simp only [formula.iff_]
-    -- simp only [formula.and_]
-    apply IsReplOfFormulaInFormula.not_
-    apply IsReplOfFormulaInFormula.imp_
-    · apply IsReplOfFormulaInFormula.imp_
-      · apply IsReplOfFormulaInFormula.same_
+    apply is_repl_of_formula_in_formula.not_
+    apply is_repl_of_formula_in_formula.imp_
+    · apply is_repl_of_formula_in_formula.imp_
+      · apply is_repl_of_formula_in_formula.same_
         rfl
-      · apply IsReplOfFormulaInFormula.not_
-        apply IsReplOfFormulaInFormula.not_
-        apply IsReplOfFormulaInFormula.forall_
-        apply IsReplOfFormulaInFormula.diff_
+      · apply is_repl_of_formula_in_formula.not_
+        apply is_repl_of_formula_in_formula.not_
+        apply is_repl_of_formula_in_formula.forall_
         · rfl
+        · apply is_repl_of_formula_in_formula.diff_
+          · rfl
+          · rfl
+    · apply is_repl_of_formula_in_formula.not_
+      apply is_repl_of_formula_in_formula.imp_
+      · apply is_repl_of_formula_in_formula.not_
+        apply is_repl_of_formula_in_formula.not_
+        apply is_repl_of_formula_in_formula.forall_
         · rfl
-    · apply IsReplOfFormulaInFormula.not_
-      apply IsReplOfFormulaInFormula.imp_
-      · apply IsReplOfFormulaInFormula.not_
-        apply IsReplOfFormulaInFormula.not_
-        apply IsReplOfFormulaInFormula.forall_
-        apply IsReplOfFormulaInFormula.diff_
-        · rfl
-        · rfl
-      · apply IsReplOfFormulaInFormula.same_
+        · apply is_repl_of_formula_in_formula.diff_
+          · rfl
+          · rfl
+      · apply is_repl_of_formula_in_formula.same_
         rfl
   · simp only [def_iff_]
     simp only [def_and_]
-    -- simp only [formula.iff_]
-    -- simp only [formula.and_]
     SC
   · simp only [def_iff_]
     simp only [def_and_]
-    -- simp only [formula.iff_]
-    -- simp only [formula.and_]
     SC
 
 
 theorem T_18_6
   (P_u P_v : Formula_)
   (u v : VarName_)
-  (h1 : Similar P_u P_v u v) :
+  (h1 : similar P_u P_v u v) :
   is_proof_v1 ((forall_ u P_u).iff_ (forall_ v P_v)) :=
   by
-  simp only [Similar] at h1
-  cases h1
-  case _ h1_left h1_right =>
-    cases h1_right
-    case _ h1_right_left h1_right_right =>
-      cases h1_right_right
-      case _ h1_right_right_left h1_right_right_right =>
-        cases h1_right_right_right
-        case _ h1_right_right_right_left h1_right_right_right_right =>
-          cases h1_right_right_right_right
-          case _ h1_right_right_right_right_left h1_right_right_right_right_right =>
-            apply is_deduct_v1.mp_ ((forall_ v P_v).imp_ (forall_ u P_u))
-            · apply is_deduct_v1.mp_ ((forall_ u P_u).imp_ (forall_ v P_v))
-              · simp only [def_iff_]
-                simp only [def_and_]
-                -- simp only [formula.iff_]
-                -- simp only [formula.and_]
-                SC
-              · apply deduction_theorem
-                simp
-                apply generalization
-                · subst h1_right_right_right_right_left
-                  apply spec
-                  · apply is_deduct_v1.assume_
-                    simp
-                  · exact h1_right_right_left
-                · intro H a1
-                  simp at a1
-                  subst a1
-                  simp only [var_is_free_in]
-                  simp
-                  intro _
-                  exact h1_left
-            · apply deduction_theorem
-              simp
-              apply generalization
-              · subst h1_right_right_right_right_right
-                apply spec
-                · apply is_deduct_v1.assume_
-                  simp
-                · exact h1_right_right_right_left
-              · intro H a1
-                simp at a1
-                subst a1
-                simp only [var_is_free_in]
-                simp
-                intro _
-                exact h1_right_left
+  simp only [similar] at h1
+  obtain ⟨h1_left, ⟨h1_right_left, ⟨h1_right_right_left, ⟨ h1_right_right_right_left, ⟨h1_right_right_right_right_left, h1_right_right_right_right_right⟩⟩⟩⟩⟩ := h1
+
+  apply is_deduct_v1.mp_ ((forall_ v P_v).imp_ (forall_ u P_u))
+  · apply is_deduct_v1.mp_ ((forall_ u P_u).imp_ (forall_ v P_v))
+    · simp only [def_iff_]
+      simp only [def_and_]
+      SC
+    · apply deduction_theorem
+      simp
+      apply generalization
+      · rw [h1_right_right_right_right_left]
+        apply spec
+        · apply is_deduct_v1.assume_
+          simp
+        · exact h1_right_right_left
+      · intro H a1
+        simp at a1
+        subst a1
+        simp only [var_is_free_in]
+        simp
+        intro _
+        exact h1_left
+  · apply deduction_theorem
+    simp
+    apply generalization
+    · rw [h1_right_right_right_right_right]
+      apply spec
+      · apply is_deduct_v1.assume_
+        simp
+      · exact h1_right_right_right_left
+    · intro H a1
+      simp at a1
+      rw [a1]
+      simp only [var_is_free_in]
+      simp
+      intro _
+      exact h1_right_left
 
 
 -- Change of bound variable
@@ -1151,8 +1106,8 @@ theorem T_18_7
   (u v : VarName_)
   (Δ : Set Formula_)
   (h1 : is_deduct_v1 Δ Q)
-  (h2 : IsReplOfFormulaInFormula (forall_ u P_u) (forall_ v P_v) Q Q')
-  (h3 : Similar P_u P_v u v) :
+  (h2 : is_repl_of_formula_in_formula (forall_ u P_u) (forall_ v P_v) Q Q')
+  (h3 : similar P_u P_v u v) :
   is_deduct_v1 Δ Q' :=
   by
   apply C_18_4 (forall_ u P_u) (forall_ v P_v) Q Q' Δ h2
@@ -1163,10 +1118,10 @@ theorem T_18_7
 theorem similar_not
   (P_u P_v : Formula_)
   (u v : VarName_)
-  (h1 : Similar P_u P_v u v) :
-  Similar P_u.not_ P_v.not_ u v :=
+  (h1 : similar P_u P_v u v) :
+  similar P_u.not_ P_v.not_ u v :=
   by
-  simp only [Similar] at *
+  simp only [similar] at *
   simp only [var_is_free_in] at *
   simp only [fast_admits_var_one_rec] at *
   simp only [fast_admits_var_one_rec_aux] at *
@@ -1177,16 +1132,13 @@ theorem similar_not
 theorem T_18_8
   (P_u P_v : Formula_)
   (u v : VarName_)
-  (h1 : Similar P_u P_v u v) :
+  (h1 : similar P_u P_v u v) :
   is_proof_v1 ((exists_ u P_u).iff_ (exists_ v P_v)) :=
   by
   simp only [def_exists_]
-  -- simp only [exists_]
   apply is_deduct_v1.mp_ ((forall_ u P_u.not_).iff_ (forall_ v P_v.not_))
   · simp only [def_iff_]
     simp only [def_and_]
-    -- simp only [formula.iff_]
-    -- simp only [formula.and_]
     SC
   · apply T_18_6
     exact similar_not P_u P_v u v h1
@@ -1198,8 +1150,8 @@ theorem T18_9
   (u v : VarName_)
   (Δ : Set Formula_)
   (h1 : is_deduct_v1 Δ Q)
-  (h2 : IsReplOfFormulaInFormula (exists_ u P_u) (exists_ v P_v) Q Q')
-  (h3 : Similar P_u P_v u v) :
+  (h2 : is_repl_of_formula_in_formula (exists_ u P_u) (exists_ v P_v) Q Q')
+  (h3 : similar P_u P_v u v) :
   is_deduct_v1 Δ Q' :=
   by
   apply C_18_4 (exists_ u P_u) (exists_ v P_v) Q Q' Δ h2
@@ -1216,9 +1168,7 @@ theorem T_19_1
   apply is_deduct_v1.mp_ ((forall_ v P).imp_ P)
   · apply is_deduct_v1.mp_ (P.imp_ (forall_ v P))
     · simp only [def_iff_]
-    -- sim only [formula.iff_]
       simp only [def_and_]
-      -- simp only [formula.and_]
       SC
     · apply is_deduct_v1.axiom_
       exact is_axiom_v1.pred_3_ v P h1
@@ -1237,8 +1187,6 @@ theorem T_19_2
   · apply is_deduct_v1.mp_ ((forall_ v (forall_ u P)).imp_ (forall_ u (forall_ v P)))
     · simp only [def_iff_]
       simp only [def_and_]
-      -- simp only [formula.iff_]
-      -- simp only [formula.and_]
       SC
     · apply T_17_10
   · apply T_17_10
@@ -1252,9 +1200,6 @@ theorem T_19_3
   simp only [def_exists_]
   simp only [def_iff_]
   simp only [def_and_]
-  -- simp only [Formula_.exists_]
-  -- simp only [formula.iff_]
-  -- simp only [formula.and_]
   SC
 
 
@@ -1272,22 +1217,18 @@ theorem T_19_4
     · apply exists_intro P u u
       · apply fast_admits_var_one_rec_self
       · simp only [fast_replace_free_var_one_rec_self]
-        apply specId v
+        apply spec_id v
         apply is_deduct_v1.assume_
         simp
     · simp
       simp only [def_exists_]
-      -- simp only [Formula_.exists_]
       simp only [var_is_free_in]
       simp
     · simp only [def_exists_]
       simp only [var_is_free_in]
-      -- simp only [exists_]
-      -- simp only [is_free_in]
       simp
   · simp
     simp only [def_exists_]
-    -- simp only [Formula_.exists_]
     simp only [var_is_free_in]
     simp
 
@@ -1302,8 +1243,6 @@ theorem T_19_5
   · apply is_deduct_v1.mp_ ((forall_ v (P.iff_ Q)).imp_ ((forall_ v P).iff_ (forall_ v Q)))
     · simp only [def_iff_]
       simp only [def_and_]
-      -- simp only [formula.iff_]
-      -- simp only [formula.and_]
       SC
     · exact T_18_1 P Q v
   · exact T_19_1 P v h1
@@ -1327,21 +1266,17 @@ theorem T_19_6_left
       · apply is_deduct_v1.mp_ (P.iff_ Q)
         · simp only [def_iff_]
           simp only [def_and_]
-          -- simp only [iff_]
-          -- simp only [and_]
           SC
-        · apply specId v
+        · apply spec_id v
           apply is_deduct_v1.assume_
           simp
       · apply is_deduct_v1.assume_
         simp
   · simp only [def_exists_]
-    -- simp only [exists_]
     simp
     simp only [var_is_free_in]
     simp
   · simp only [def_exists_]
-    -- simp only [exists_]
     simp only [var_is_free_in]
     simp
 
@@ -1360,10 +1295,8 @@ theorem T_19_6_right
     · apply is_deduct_v1.mp_ (P.iff_ Q)
       · simp only [def_iff_]
         simp only [def_and_]
-        -- simp only [iff_]
-        -- simp only [and_]
         SC
-      · apply specId v
+      · apply spec_id v
         apply is_deduct_v1.assume_
         simp
     · simp
@@ -1381,9 +1314,6 @@ theorem T_19_6
     · simp only [def_exists_]
       simp only [def_iff_]
       simp only [def_and_]
-      -- simp only [exists_]
-      -- simp only [iff_]
-      -- simp only [and_]
       SC
     · apply T_19_6_right
   · apply T_19_6_left
@@ -1396,14 +1326,14 @@ theorem T_19_TS_21_left
   is_proof_v1 ((forall_ v (P.imp_ Q)).imp_ (P.imp_ (forall_ v Q))) :=
   by
   apply C_18_4 (forall_ v P) P ((forall_ v (P.imp_ Q)).imp_ ((forall_ v P).imp_ (forall_ v Q)))
-  · apply IsReplOfFormulaInFormula.imp_
-    · apply IsReplOfFormulaInFormula.same_
+  · apply is_repl_of_formula_in_formula.imp_
+    · apply is_repl_of_formula_in_formula.same_
       rfl
-    · apply IsReplOfFormulaInFormula.imp_
-      · apply IsReplOfFormulaInFormula.diff_
+    · apply is_repl_of_formula_in_formula.imp_
+      · apply is_repl_of_formula_in_formula.diff_
         · rfl
         · rfl
-      · apply IsReplOfFormulaInFormula.same_
+      · apply is_repl_of_formula_in_formula.same_
         rfl
   · exact T_19_1 P v h1
   · apply is_deduct_v1.axiom_
@@ -1420,7 +1350,7 @@ theorem T_19_TS_21_right
   simp
   apply generalization
   · apply deduction_theorem
-    apply specId v
+    apply spec_id v
     apply is_deduct_v1.mp_ P
     · apply is_deduct_v1.assume_
       simp
@@ -1444,8 +1374,6 @@ theorem T_19_TS_21
   · apply is_deduct_v1.mp_ ((P.imp_ (forall_ v Q)).imp_ (forall_ v (P.imp_ Q)))
     · simp only [def_iff_]
       simp only [def_and_]
-      -- simp only [formula.iff_]
-      -- simp only [formula.and_]
       SC
     · exact T_19_TS_21_right P Q v h1
   · exact T_19_TS_21_left P Q v h1
@@ -1461,16 +1389,14 @@ theorem T_21_1
       · apply is_deduct_v1.mp_ (((eq_ y y).and_ (eq_ x y)).imp_ ((eq_ y x).iff_ (eq_ y y)))
         · simp only [def_iff_]
           simp only [def_and_]
-          -- simp only [formula.iff_]
-          -- simp only [formula.and_]
           SC
-        · apply specId y
-          apply specId y
-          apply specId x
-          apply specId y
+        · apply spec_id y
+          apply spec_id y
+          apply spec_id x
+          apply spec_id y
           apply is_deduct_v1.axiom_
           exact is_axiom_v1.eq_2_eq_ y x y y
-      · apply specId y
+      · apply spec_id y
         apply is_deduct_v1.axiom_
         exact is_axiom_v1.eq_1_ y
     · intro H a1
@@ -1490,16 +1416,14 @@ theorem T_21_2
         · apply is_deduct_v1.mp_ (((eq_ x y).and_ (eq_ z z)).imp_ ((eq_ x z).iff_ (eq_ y z)))
           · simp only [def_iff_]
             simp only [def_and_]
-            -- simp only [formula.iff_]
-            -- simp only [formula.and_]
             SC
-          · apply specId z
-            apply specId y
-            apply specId z
-            apply specId x
+          · apply spec_id z
+            apply spec_id y
+            apply spec_id z
+            apply spec_id x
             apply is_deduct_v1.axiom_
             exact is_axiom_v1.eq_2_eq_ x z y z
-        · apply specId z
+        · apply spec_id z
           apply is_deduct_v1.axiom_
           exact is_axiom_v1.eq_1_ z
       · intro H a1
@@ -1521,26 +1445,15 @@ theorem T_21_8
   induction h1
   case true_ =>
     simp only [def_iff_]
-    -- simp only [formula.iff_]
     simp only [def_and_]
-    -- simp only [formula.and_]
     SC
-  case pred_const_ name n args_u args_v
-    h1_1 =>
-    apply
-      is_deduct_v1.mp_
-        ((eq_ r s).imp_ ((pred_const_ name (List.ofFn args_u)).iff_ (pred_const_ name (List.ofFn args_v))))
+  case pred_const_ name n args_u args_v h1_1 =>
+    apply is_deduct_v1.mp_ ((eq_ r s).imp_ ((pred_const_ name (List.ofFn args_u)).iff_ (pred_const_ name (List.ofFn args_v))))
     · SC
-    · apply
-        is_deduct_v1.mp_ ((eq_ r s).imp_ (And_ (List.ofFn fun (i : Fin n) => eq_ (args_u i) (args_v i))))
-      · apply
-          is_deduct_v1.mp_
-            ((And_ (List.ofFn fun (i : Fin n) => eq_ (args_u i) (args_v i))).imp_
-              ((pred_const_ name (List.ofFn args_u)).iff_ (pred_const_ name (List.ofFn args_v))))
+    · apply is_deduct_v1.mp_ ((eq_ r s).imp_ (And_ (List.ofFn fun (i : Fin n) => eq_ (args_u i) (args_v i))))
+      · apply is_deduct_v1.mp_ ((And_ (List.ofFn fun (i : Fin n) => eq_ (args_u i) (args_v i))).imp_ ((pred_const_ name (List.ofFn args_u)).iff_ (pred_const_ name (List.ofFn args_v))))
         · simp only [def_iff_]
-          -- simp only [formula.iff_]
           simp only [def_and_]
-          -- simp only [formula.and_]
           SC
         · apply Forall_spec_id' (List.ofFn args_v)
           apply Forall_spec_id' (List.ofFn args_u)
@@ -1555,32 +1468,24 @@ theorem T_21_8
           SC
         case _ n ih =>
           simp
-          apply
-            is_deduct_v1.mp_
-              ((eq_ r s).imp_
-                (List.foldr and_ true_
-                  (List.ofFn fun (i : Fin n) => eq_ (args_u i.succ) (args_v i.succ))))
+          apply is_deduct_v1.mp_ ((eq_ r s).imp_ (List.foldr and_ true_ (List.ofFn fun (i : Fin n) => eq_ (args_u i.succ) (args_v i.succ))))
           · apply is_deduct_v1.mp_ ((eq_ r s).imp_ (eq_ (args_u 0) (args_v 0)))
             · simp only [def_and_]
-              -- simp only [formula.and_]
               SC
             · specialize h1_1 0
               cases h1_1
               case _ c1 =>
                 apply is_deduct_v1.mp_ (eq_ (args_u 0) (args_v 0))
-                case _ =>
-                  SC
-                case _ =>
-                  simp only [c1]
-                  apply specId (args_v 0)
+                · SC
+                · simp only [c1]
+                  apply spec_id (args_v 0)
                   apply is_deduct_v1.axiom_
                   apply is_axiom_v1.eq_1_
               case _ c1 =>
-                cases c1
-                case _ c1_left c1_right =>
-                  subst c1_left
-                  subst c1_right
-                  SC
+                obtain ⟨c1_left, c1_right⟩ := c1
+                subst c1_left
+                subst c1_right
+                SC
           · apply ih
             intro i
             apply h1_1
@@ -1590,64 +1495,56 @@ theorem T_21_8
     specialize h1_ih h2 h3
     apply is_deduct_v1.mp_ ((eq_ r s).imp_ (P_u.iff_ P_v))
     · simp only [def_iff_]
-      -- simp only [formula.iff_]
       simp only [def_and_]
-      -- simp only [formula.and_]
       SC
     · exact h1_ih
   case imp_ P_u Q_u P_v Q_v h1_1 h1_2 h1_ih_1
     h1_ih_2 =>
     simp only [var_is_bound_in] at h2
-    push_neg at h2
-    cases h2
-    case intro h2_left h2_right =>
-      simp only [var_is_bound_in] at h3
-      push_neg at h3
-      cases h3
-      case intro h3_left h3_right =>
-        specialize h1_ih_1 h2_left h3_left
-        specialize h1_ih_2 h2_right h3_right
-        apply is_deduct_v1.mp_ ((eq_ r s).imp_ (Q_u.iff_ Q_v))
-        · apply is_deduct_v1.mp_ ((eq_ r s).imp_ (P_u.iff_ P_v))
-          · simp only [def_iff_]
-            -- simp only [formula.iff_]
-            simp only [def_and_]
-            -- simp only [formula.and_]
-            SC
-          · exact h1_ih_1
-        · exact h1_ih_2
+    simp at h2
+    obtain ⟨h2_left, h2_right⟩ := h2
+    simp only [var_is_bound_in] at h3
+    simp at h3
+    obtain ⟨h3_left, h3_right⟩ := h3
+    specialize h1_ih_1 h2_left h3_left
+    specialize h1_ih_2 h2_right h3_right
+    apply is_deduct_v1.mp_ ((eq_ r s).imp_ (Q_u.iff_ Q_v))
+    · apply is_deduct_v1.mp_ ((eq_ r s).imp_ (P_u.iff_ P_v))
+      · simp only [def_iff_]
+        simp only [def_and_]
+        SC
+      · exact h1_ih_1
+    · exact h1_ih_2
   case forall_ x P_u P_v h1_1 h1_ih =>
     simp only [var_is_bound_in] at h2
-    push_neg at h2
-    cases h2
-    case _ h2_left h2_right =>
-      simp only [var_is_bound_in] at h3
-      push_neg at h3
-      cases h3
-      case _ h3_left h3_right =>
-        apply deduction_theorem
-        simp
-        apply is_deduct_v1.mp_ (forall_ x (P_u.iff_ P_v))
-        · apply proof_imp_deduct
-          apply T_18_1
-        · apply is_deduct_v1.mp_ (eq_ r s)
-          · apply proof_imp_deduct
-            apply is_deduct_v1.mp_ (forall_ x ((eq_ r s).imp_ (P_u.iff_ P_v)))
-            · apply T_19_TS_21_left
-              · -- simp only [formula.eq_]
-                simp only [var_is_free_in]
-                push_neg
-                constructor
-                · simp only [ne_comm]
-                  exact h2_left
-                · simp only [ne_comm]
-                  exact h3_left
-            · apply generalization
-              · exact h1_ih h2_right h3_right
-              · intro H a1
-                simp at a1
-          · apply is_deduct_v1.assume_
+    simp at h2
+    obtain ⟨h2_left, h2_right⟩ := h2
+
+    simp only [var_is_bound_in] at h3
+    simp at h3
+    obtain ⟨h3_left, h3_right⟩ := h3
+    apply deduction_theorem
+    simp
+    apply is_deduct_v1.mp_ (forall_ x (P_u.iff_ P_v))
+    · apply proof_imp_deduct
+      apply T_18_1
+    · apply is_deduct_v1.mp_ (eq_ r s)
+      · apply proof_imp_deduct
+        apply is_deduct_v1.mp_ (forall_ x ((eq_ r s).imp_ (P_u.iff_ P_v)))
+        · apply T_19_TS_21_left
+          · simp only [var_is_free_in]
             simp
+            constructor
+            · simp only [ne_comm]
+              exact h2_left
+            · simp only [ne_comm]
+              exact h3_left
+        · apply generalization
+          · exact h1_ih h2_right h3_right
+          · intro H a1
+            simp at a1
+      · apply is_deduct_v1.assume_
+        simp
   all_goals
     sorry
 
