FOL/NV/ReplaceSubFormula.lean
@@ -250,4 +250,414 @@ example
     tauto
 
 
-#lint
+-------------------------------------------------------------------------------
+
+
+/--
+  is_repl_of_var_in_list_fun u v l_u l_v := True if and only if l_v is the result of replacing one or more specified occurrences (but not necessarily all occurrences) of u in l_u by occurrences of v.
+-/
+def is_repl_of_var_in_list_fun
+  (u v : VarName_) :
+  List VarName_ → List VarName_ → Prop
+  | [], [] => True
+  | hd_u :: tl_u, hd_v :: tl_v =>
+    (hd_u = hd_v ∨ (hd_u = u ∧ hd_v = v)) ∧ is_repl_of_var_in_list_fun u v tl_u tl_v
+  | _, _ => False
+
+
+inductive is_repl_of_var_in_list
+  (u v : VarName_) :
+  List VarName_ → List VarName_ → Prop
+  | nil_ : is_repl_of_var_in_list u v [] []
+
+  | cons_same_
+    (hd_u hd_v : VarName_)
+    (tl_u tl_v : List VarName_) :
+    hd_u = hd_v →
+    is_repl_of_var_in_list u v tl_u tl_v →
+    is_repl_of_var_in_list u v (hd_u :: tl_u) (hd_v :: tl_v)
+
+  | cons_diff_
+    (hd_u hd_v : VarName_)
+    (tl_u tl_v : List VarName_) :
+    hd_u = u →
+    hd_v = v →
+    is_repl_of_var_in_list u v tl_u tl_v →
+    is_repl_of_var_in_list u v (hd_u :: tl_u) (hd_v :: tl_v)
+
+
+lemma is_repl_of_var_in_list_fun_imp_is_repl_of_var_in_list
+  (u v : VarName_)
+  (us vs : List VarName_)
+  (h1 : is_repl_of_var_in_list_fun u v us vs) :
+  is_repl_of_var_in_list u v us vs :=
+  by
+  induction us generalizing vs
+  case nil =>
+    cases vs
+    case nil =>
+      apply is_repl_of_var_in_list.nil_
+    case cons hd_v tl_v =>
+      simp only [is_repl_of_var_in_list_fun] at h1
+  case cons hd_u tl_u ih_u =>
+    cases vs
+    case nil =>
+      simp only [is_repl_of_var_in_list_fun] at h1
+    case cons hd_v tl_v =>
+      simp only [is_repl_of_var_in_list_fun] at h1
+      obtain ⟨h1_left, h1_right⟩ := h1
+      cases h1_left
+      case _ h1_left =>
+        apply is_repl_of_var_in_list.cons_same_
+        · exact h1_left
+        · apply ih_u
+          exact h1_right
+      case _ h1_left =>
+        obtain ⟨h1_left_left, h1_left_right⟩ := h1_left
+        apply is_repl_of_var_in_list.cons_diff_
+        · exact h1_left_left
+        · exact h1_left_right
+        · apply ih_u
+          exact h1_right
+
+
+lemma is_repl_of_var_in_list_imp_is_repl_of_var_in_list_fun
+  (u v : VarName_)
+  (us vs : List VarName_)
+  (h1 : is_repl_of_var_in_list u v us vs) :
+  is_repl_of_var_in_list_fun u v us vs :=
+  by
+  induction h1
+  all_goals
+    simp only [is_repl_of_var_in_list_fun]
+  all_goals
+    tauto
+
+
+-------------------------------------------------------------------------------
+
+
+/--
+  is_repl_of_var_in_formula_fun u v P_u P_v := True if and only if P_v is the result of replacing one or more specified occurrences (but not necessarily all occurrences) of u in P_u by occurrences of v.
+-/
+def is_repl_of_var_in_formula_fun
+  (u v : VarName_) :
+  Formula_ → Formula_ → Prop
+  | pred_var_ name_u args_u, pred_var_ name_v args_v =>
+      name_u = name_v ∧ is_repl_of_var_in_list_fun u v args_u args_v
+  | pred_const_ name_u args_u, pred_const_ name_v args_v =>
+      name_u = name_v ∧ is_repl_of_var_in_list_fun u v args_u args_v
+  | eq_ x_u y_u, eq_ x_v y_v =>
+      is_repl_of_var_in_list_fun u v [x_u, y_u] [x_v, y_v]
+  | true_, true_ => True
+  | false_, false_ => True
+  | not_ P_u, not_ P_v => is_repl_of_var_in_formula_fun u v P_u P_v
+  | imp_ P_u Q_u, imp_ P_v Q_v =>
+      is_repl_of_var_in_formula_fun u v P_u P_v ∧
+      is_repl_of_var_in_formula_fun u v Q_u Q_v
+  | and_ P_u Q_u, and_ P_v Q_v =>
+      is_repl_of_var_in_formula_fun u v P_u P_v ∧
+      is_repl_of_var_in_formula_fun u v Q_u Q_v
+  | or_ P_u Q_u, or_ P_v Q_v =>
+      is_repl_of_var_in_formula_fun u v P_u P_v ∧
+      is_repl_of_var_in_formula_fun u v Q_u Q_v
+  | iff_ P_u Q_u, iff_ P_v Q_v =>
+      is_repl_of_var_in_formula_fun u v P_u P_v ∧
+      is_repl_of_var_in_formula_fun u v Q_u Q_v
+  | forall_ x P_u, forall_ x' P_v =>
+      x = x' ∧ is_repl_of_var_in_formula_fun u v P_u P_v
+  | exists_ x P_u, exists_ x' P_v =>
+      x = x' ∧ is_repl_of_var_in_formula_fun u v P_u P_v
+  | _, _ => False
+
+
+/--
+  `is_repl_of_var_in_formula u v P_u P_v` := True if and only if `P_v` is the result of replacing one or more specified occurrences (but not necessarily all occurrences) of `u` in `P_u` by occurrences of `v`.
+-/
+inductive is_repl_of_var_in_formula
+  (u v : VarName_) :
+  Formula_ → Formula_ → Prop
+  | pred_const_
+    (name_u name_v : PredName_)
+    (args_u args_v : List VarName_) :
+    name_u = name_v →
+    is_repl_of_var_in_list u v args_u args_v →
+    is_repl_of_var_in_formula u v (pred_const_ name_u args_u) (pred_const_ name_v args_v)
+
+  | pred_var_
+    (name_u name_v : PredName_)
+    (args_u args_v : List VarName_) :
+    name_u = name_v →
+    is_repl_of_var_in_list u v args_u args_v →
+    is_repl_of_var_in_formula u v (pred_var_ name_u args_u) (pred_var_ name_v args_v)
+
+  | eq_
+    (x_u y_u x_v y_v : VarName_) :
+    ((x_u = x_v) ∨ (x_u = u ∧ x_v = v)) →
+    ((y_u = y_v) ∨ (y_u = u ∧ y_v = v)) →
+    is_repl_of_var_in_formula u v (eq_ x_u y_u) (eq_ x_v y_v)
+
+  | true_ :
+    is_repl_of_var_in_formula u v true_ true_
+
+  | false_ :
+    is_repl_of_var_in_formula u v false_ false_
+
+  | not_
+    (P_u P_v : Formula_) :
+    is_repl_of_var_in_formula u v P_u P_v →
+    is_repl_of_var_in_formula u v P_u.not_ P_v.not_
+
+  | imp_
+    (P_u Q_u : Formula_)
+    (P_v Q_v : Formula_) :
+    is_repl_of_var_in_formula u v P_u P_v →
+    is_repl_of_var_in_formula u v Q_u Q_v →
+    is_repl_of_var_in_formula u v (P_u.imp_ Q_u) (P_v.imp_ Q_v)
+
+  | and_
+    (P_u Q_u : Formula_)
+    (P_v Q_v : Formula_) :
+    is_repl_of_var_in_formula u v P_u P_v →
+    is_repl_of_var_in_formula u v Q_u Q_v →
+    is_repl_of_var_in_formula u v (P_u.and_ Q_u) (P_v.and_ Q_v)
+
+  | or_
+    (P_u Q_u : Formula_)
+    (P_v Q_v : Formula_) :
+    is_repl_of_var_in_formula u v P_u P_v →
+    is_repl_of_var_in_formula u v Q_u Q_v →
+    is_repl_of_var_in_formula u v (P_u.or_ Q_u) (P_v.or_ Q_v)
+
+  | iff_
+    (P_u Q_u : Formula_)
+    (P_v Q_v : Formula_) :
+    is_repl_of_var_in_formula u v P_u P_v →
+    is_repl_of_var_in_formula u v Q_u Q_v →
+    is_repl_of_var_in_formula u v (P_u.iff_ Q_u) (P_v.iff_ Q_v)
+
+  | forall_
+    (x_u x_v : VarName_)
+    (P_u P_v : Formula_) :
+    x_u = x_v →
+    is_repl_of_var_in_formula u v P_u P_v →
+    is_repl_of_var_in_formula u v (forall_ x_u P_u) (forall_ x_v P_v)
+
+  | exists_
+    (x_u x_v : VarName_)
+    (P_u P_v : Formula_) :
+    x_u = x_v →
+    is_repl_of_var_in_formula u v P_u P_v →
+    is_repl_of_var_in_formula u v (exists_ x_u P_u) (exists_ x_v P_v)
+
+
+theorem extracted_10
+  (u v : VarName_)
+  (n : ℕ)
+  (args_u args_v : Fin n → VarName_)
+  (h1 : ∀ (i : Fin n), args_u i = args_v i ∨ args_u i = u ∧ args_v i = v) :
+  is_repl_of_var_in_list_fun u v (List.ofFn args_u) (List.ofFn args_v) :=
+  by
+  induction n
+  case zero =>
+    simp_all only [IsEmpty.forall_iff, List.ofFn_zero]
+    unfold is_repl_of_var_in_list_fun
+    trivial
+  case succ m ih =>
+    simp_all only [List.ofFn_succ]
+    unfold is_repl_of_var_in_list_fun
+    constructor
+    · apply h1
+    · exact ih (fun i => args_u i.succ) (fun i => args_v i.succ) fun i => h1 i.succ
+
+
+example
+  (u v : VarName_)
+  (F F' : Formula_)
+  (h1 : is_repl_of_var_in_formula u v F F') :
+  is_repl_of_var_in_formula_fun u v F F' :=
+  by
+  induction h1
+  case
+      pred_const_ name_u name_v args_u args_v ih_1 ih_2
+    | pred_var_ name_u name_v args_u args_v ih_1 ih_2 =>
+    unfold is_repl_of_var_in_formula_fun
+    constructor
+    · exact ih_1
+    · apply is_repl_of_var_in_list_imp_is_repl_of_var_in_list_fun
+      exact ih_2
+  case eq_ x_u y_u x_v y_v ih_1 ih_2 =>
+    unfold is_repl_of_var_in_formula_fun
+    simp only [is_repl_of_var_in_list_fun]
+    tauto
+  case true_ =>
+    simp only [is_repl_of_var_in_formula_fun]
+  case false_ =>
+    simp only [is_repl_of_var_in_formula_fun]
+  case not_ P_u P_v ih_1 ih_2 =>
+    unfold is_repl_of_var_in_formula_fun
+    exact ih_2
+  case
+      imp_ P_u Q_u P_v Q_v ih_1 ih_2 ih_3 ih_4
+    | and_ P_u Q_u P_v Q_v ih_1 ih_2 ih_3 ih_4
+    | or_ P_u Q_u P_v Q_v ih_1 ih_2 ih_3 ih_4
+    | iff_ P_u Q_u P_v Q_v ih_1 ih_2 ih_3 ih_4 =>
+    unfold is_repl_of_var_in_formula_fun
+    tauto
+  case
+      forall_ x P_u P_v ih_1 ih_2
+    | exists_ x P_u P_v ih_1 ih_2 =>
+    unfold is_repl_of_var_in_formula_fun
+    tauto
+
+
+example
+  (u v : VarName_)
+  (F F' : Formula_)
+  (h1 : is_repl_of_var_in_formula_fun u v F F') :
+  is_repl_of_var_in_formula u v F F' :=
+  by
+  induction F generalizing F'
+  all_goals
+    cases F'
+  case
+      pred_const_.pred_const_ name_u args_u name_v args_v
+    | pred_var_.pred_var_ name_u args_u name_v args_v =>
+    simp only [is_repl_of_var_in_formula_fun] at h1
+    obtain ⟨h1_left, h1_right⟩ := h1
+
+    first
+      | apply is_repl_of_var_in_formula.pred_const_
+      | apply is_repl_of_var_in_formula.pred_var_
+    · exact h1_left
+    · apply is_repl_of_var_in_list_fun_imp_is_repl_of_var_in_list
+      exact h1_right
+  case eq_.eq_ x_u y_u x_v y_v =>
+    simp only [is_repl_of_var_in_formula_fun] at h1
+    simp only [is_repl_of_var_in_list_fun] at h1
+
+    apply is_repl_of_var_in_formula.eq_
+    · tauto
+    · tauto
+  case true_.true_ =>
+    apply is_repl_of_var_in_formula.true_
+  case false_.false_ =>
+    apply is_repl_of_var_in_formula.false_
+  case not_.not_ phi_u ih phi_v =>
+    simp only [is_repl_of_var_in_formula_fun] at h1
+
+    apply is_repl_of_var_in_formula.not_
+    tauto
+  case
+      imp_.imp_ phi_u psi_u ih_1 ih_2 phi_v psi_v
+    | and_.and_ phi_u psi_u ih_1 ih_2 phi_v psi_v
+    | or_.or_ phi_u psi_u ih_1 ih_2 phi_v psi_v
+    | iff_.iff_ phi_u psi_u ih_1 ih_2 phi_v psi_v =>
+    simp only [is_repl_of_var_in_formula_fun] at h1
+    obtain ⟨h1_left, h1_right⟩ := h1
+
+    first
+      | apply is_repl_of_var_in_formula.imp_
+      | apply is_repl_of_var_in_formula.and_
+      | apply is_repl_of_var_in_formula.or_
+      | apply is_repl_of_var_in_formula.iff_
+    · tauto
+    · tauto
+  case
+      forall_.forall_ x_u phi_u ih x_v phi_v
+    | exists_.exists_ x_u phi_u ih x_v phi_v =>
+    simp only [is_repl_of_var_in_formula_fun] at h1
+    obtain ⟨h1_left, h1_right⟩ := h1
+
+    first
+      | apply is_repl_of_var_in_formula.forall_
+      | apply is_repl_of_var_in_formula.exists_
+    · exact h1_left
+    · apply ih
+      exact h1_right
+  all_goals
+    simp only [is_repl_of_var_in_formula_fun] at h1
+
+
+-------------------------------------------------------------------------------
+
+
+/--
+  IsReplOfVarInFormula u v P_u P_v := True if and only if P_v is the result of replacing one or more specified occurrences (but not necessarily all occurrences) of u in P_u by occurrences of v.
+-/
+inductive IsReplOfVarInFormula
+  (u v : VarName_) :
+  Formula_ → Formula_ → Prop
+  | pred_const_
+    (name : PredName_)
+    (n : ℕ)
+    (args_u args_v : Fin n → VarName_) :
+    (∀ (i : Fin n), (args_u i = args_v i) ∨ (args_u i = u ∧ args_v i = v)) →
+    IsReplOfVarInFormula u v (pred_const_ name (List.ofFn args_u)) (pred_const_ name (List.ofFn args_v))
+
+  | pred_var_
+    (name : PredName_)
+    (n : ℕ)
+    (args_u args_v : Fin n → VarName_) :
+    (∀ (i : Fin n), (args_u i = args_v i) ∨ (args_u i = u ∧ args_v i = v)) →
+    IsReplOfVarInFormula u v (pred_var_ name (List.ofFn args_u)) (pred_var_ name (List.ofFn args_v))
+
+  | eq_
+    (x_u y_u x_v y_v : VarName_) :
+    ((x_u = x_v) ∨ (x_u = u ∧ x_v = v)) →
+    ((y_u = y_v) ∨ (y_u = u ∧ y_v = v)) →
+    IsReplOfVarInFormula u v (eq_ x_u y_u) (eq_ x_v y_v)
+
+  | true_ :
+    IsReplOfVarInFormula u v true_ true_
+
+  | false_ :
+    IsReplOfVarInFormula u v false_ false_
+
+  | not_
+    (P_u P_v : Formula_) :
+    IsReplOfVarInFormula u v P_u P_v →
+    IsReplOfVarInFormula u v P_u.not_ P_v.not_
+
+  | imp_
+    (P_u Q_u : Formula_)
+    (P_v Q_v : Formula_) :
+    IsReplOfVarInFormula u v P_u P_v →
+    IsReplOfVarInFormula u v Q_u Q_v →
+    IsReplOfVarInFormula u v (P_u.imp_ Q_u) (P_v.imp_ Q_v)
+
+  | and_
+    (P_u Q_u : Formula_)
+    (P_v Q_v : Formula_) :
+    IsReplOfVarInFormula u v P_u P_v →
+    IsReplOfVarInFormula u v Q_u Q_v →
+    IsReplOfVarInFormula u v (P_u.and_ Q_u) (P_v.and_ Q_v)
+
+  | or_
+    (P_u Q_u : Formula_)
+    (P_v Q_v : Formula_) :
+    IsReplOfVarInFormula u v P_u P_v →
+    IsReplOfVarInFormula u v Q_u Q_v →
+    IsReplOfVarInFormula u v (P_u.or_ Q_u) (P_v.or_ Q_v)
+
+  | iff_
+    (P_u Q_u : Formula_)
+    (P_v Q_v : Formula_) :
+    IsReplOfVarInFormula u v P_u P_v →
+    IsReplOfVarInFormula u v Q_u Q_v →
+    IsReplOfVarInFormula u v (P_u.iff_ Q_u) (P_v.iff_ Q_v)
+
+  | forall_
+    (x : VarName_)
+    (P_u P_v : Formula_) :
+    IsReplOfVarInFormula u v P_u P_v →
+    IsReplOfVarInFormula u v (forall_ x P_u) (forall_ x P_v)
+
+  | exists_
+    (x : VarName_)
+    (P_u P_v : Formula_) :
+    IsReplOfVarInFormula u v P_u P_v →
+    IsReplOfVarInFormula u v (exists_ x P_u) (exists_ x P_v)
+
+
+--#lint
